\input{preamble.sty}

\begin{document}

\section{Preliminaries}

Skipped due to triviality.

\section{Categories}

\subsection{Basic definitions}

\begin{enumerate}
    \item Prove that sets (as objects) and injective functions (as arrows) form a category with functional composition as the composition operation \(c\).
          \begin{solution}
              Take \(id_A\) to be \(x \mapsto x\), then \(\id_A \circ f = f\) and \(g \circ \id_A = g\) is trivial. The last thing to check is that \(g \circ f\) is injective, that is, whenever \(s \neq s'\), then \(g(f(s)) \neq g(f(s'))\). By injectivity of \(f\), we have \(f(s) \neq f(s')\) and by injectivity of \(g\) we have \(g(f(s)) \neq g(f(s'))\).
          \end{solution}
    \item Do the same as Exercise 1 for sets and surjective functions.
          \begin{solution}
              Let \(f : A \to B, g : B \to C\) be injective functions. Then \(f(A) = B, g(B) = C \Rightarrow g(f(A)) = C\).
          \end{solution}
    \item Show that composition of relations (2.1.14) is associative.
          \begin{solution}
              Let \(\alpha, \beta, \gamma\) be relations from \(A\) to \(B\), from \(B\) to \(C\) and from \(C\) to \(D\).
              \begin{align*}
                  \alpha \circ \beta \circ \gamma
                   & = \{(a, c) \mid \exists b : (a, b) \in \alpha, (b, c) \in \beta\} \circ \gamma          \\
                   & = \{(a, d) \mid \exists b, c : (a, b) \in \alpha, (b, c) \in \beta, (c, d) \in \gamma\} \\
                   & = \alpha \circ (\beta \circ \gamma)
              \end{align*}
          \end{solution}
    \item Prove the following for any arrow \(u : A \to A\) of a category \(\mathcal{C}\). It follows from these facts that C--3 and C--4 of 2.1.3. characterize the identity arrows of a category.
          \begin{enumerate}
              \item If \(g \circ u = g\) for every object \(B\) of \(\mathcal{C}\) and arrow \(g : A \to B\), then \(u = \id_A\).
              \item If \(u \circ h = h\) for every object \(C\) of \(\mathcal{C}\) and arrow \(h : C \to A\), then \(u = \id_A\).
          \end{enumerate}
          \begin{solution}\itemfix
              \begin{enumerate}
                  \item \(\id_A \circ u \defeq u\), but also \(\id_A \circ u = \id_A\) by assumption. \(\Rightarrow u = \id_A\).
                  \item \(u \circ \id_A \defeq u\), but also \(u \circ \id_A = \id_A\) by assumption. \(\Rightarrow u = \id_A\).
              \end{enumerate}
          \end{solution}
\end{enumerate}

\subsection{Functional programming languages}

\begin{enumerate}
    \item \(\texttt{nonzero}: \texttt{NAT} \to \texttt{BOOLEAN}\), subject to equations \(\texttt{nonzero} \circ \texttt{succ} = \texttt{false}\) and \(\texttt{nonzero} \circ \texttt{succ} = \texttt{true}\).
\end{enumerate}

\end{document}
